transformations/Moore2Mealy/Moore2Mealy.v
@@ -50,13 +50,13 @@ Definition Moore2Mealy' :=
               Mealy.TransitionSourceReference //
               (fun tls _ m moore_tr mealy_tr =>
                 maybeBuildTransitionSource mealy_tr
-                  (maybeResolve tls m "s" Mealy.StateClass 
+                  (maybeResolve tls "s" Mealy.StateClass 
                     (maybeSingleton (Moore.Transition_getSourceObject moore_tr m)))) ;
             LINK 
               Mealy.TransitionTargetReference //
               (fun tls _ m moore_tr mealy_tr =>
                 maybeBuildTransitionTarget mealy_tr
-                  (maybeResolve tls m "s" Mealy.StateClass 
+                  (maybeResolve tls "s" Mealy.StateClass 
                     (maybeSingleton (Moore.Transition_getTargetObject moore_tr m)))) 
           >>>
       ]
