transformations/TT2BDD/TT2BDDAbstract.v
@@ -105,7 +105,7 @@ Definition TT2BDD :=
           (fun tls i m col output => 
             ulv <- (upper_level col);
             ucol <- locate m ulv;
-            parent <- resolveIter tls m "node" [ucol] ((div_roundup i 2)-1);
+            parent <- resolveIter tls "node" [ucol] ((div_roundup i 2)-1);
             return [BuildBDDEdge output parent])
       ]
     ) ;
@@ -119,7 +119,7 @@ Definition TT2BDD :=
             col <- locate m height;             (* get node of depth *)
             row <- hd_error sp;
             input <- (Row_Input row);
-            parent <- resolveIter tls m "node" [col] ((div_roundup (semantic input) 2)-1);   (* attach output to the corresponding leaf node*)
+            parent <- resolveIter tls "node" [col] ((div_roundup (semantic input) 2)-1);   (* attach output to the corresponding leaf node*)
             return [BuildBDDEdge output parent])
       ]
     )
